More progress on hand-translated specs

src/CertifiedExtraction/Benchmarks/QueryStructureWrappers.v
@@ -8,12 +8,6 @@ Require Import CertifiedExtraction.Core.
 Require Import Bedrock.Platform.Facade.examples.QsADTs.
 Require Import Bedrock.Platform.Facade.examples.TuplesF.
 
-(* Inductive ADTValue := *)
-(* | Tuple (t : tupl) *)
-(* | List (ts : list tupl) *)
-(* | Tuples0 (len : W) (ts : tuples) *)
-(* | Tuples1 (len key : W) (ts : tuples). *)
-
 Require Import CertifiedExtraction.Utils.
 
 Require Import Bedrock.Memory.
@@ -48,18 +42,29 @@ Definition IndexedElement_TupleToListW {N} (element: FiatElement N) : BedrockEle
   {| elementIndex := element.(IndexedEnsembles.elementIndex);
      indexedElement := TupleToListW element.(IndexedEnsembles.indexedElement) |}.
 
-(* Fixpoint ListWToilist2 (l : list W) : ilist2.ilist2 (B := fun x => x) (MakeVectorOfW (List.length l)) := *)
-(*   match l as l0 return (ilist2.ilist2 (MakeVectorOfW (Datatypes.length l0))) with *)
-(*   | nil => ilist2.inil2 *)
-(*   | x :: x0 => ilist2.icons2 x (ListWToilist2 x0) *)
-(*   end. *)
+Fixpoint ListWToilist2 (l : list W) : ilist2.ilist2 (B := fun x => x) (MakeVectorOfW (List.length l)) :=
+  match l as l0 return (ilist2.ilist2 (MakeVectorOfW (Datatypes.length l0))) with
+  | nil => ilist2.inil2
+  | x :: x0 => ilist2.icons2 x (ListWToilist2 x0)
+  end.
 
-(* Definition ListWToTuple (l: list W) : @RawTuple (MakeWordHeading (List.length l)) := *)
-(*   ListWToilist2 l. *)
+Definition ListWToTuple (l: list W) : @RawTuple (MakeWordHeading (List.length l)) :=
+  ListWToilist2 l.
 
-(* Definition IndexedElement_ListWToTuple (element: @IndexedElement (list W)) := *)
-(*   {| elementIndex := element.(elementIndex); *)
-(*      indexedElement := ListWToTuple element.(indexedElement) |}. *)
+Definition IndexedElement_ListWToTuple (element: @IndexedElement (list W)) : FiatElement (List.length (indexedElement element)) :=
+  {| IndexedEnsembles.elementIndex := element.(elementIndex);
+     IndexedEnsembles.indexedElement := ListWToTuple element.(indexedElement) |}.
+
+Lemma IndexedElement_RoundTrip :
+  forall l, IndexedElement_TupleToListW (IndexedElement_ListWToTuple l) = l.
+Proof.
+  destruct l.
+  induction indexedElement; simpl.
+  - reflexivity.
+  - unfold IndexedElement_ListWToTuple, IndexedElement_TupleToListW in *. simpl in *.
+    f_equal. inversion IHindexedElement. rewrite H0. unfold TupleToListW in *.
+    simpl. f_equal. compute in *. rewrite H0. reflexivity.
+Qed.
 
 Definition RelatedIndexedTupleAndListW {N} (l: BedrockElement) (tup: FiatElement N) :=
   l.(elementIndex) = tup.(IndexedEnsembles.elementIndex) /\
@@ -119,7 +124,7 @@ Ltac Wrapper_t :=
   abstract (intros * H; inversion H; subst; clear H; f_equal;
             eauto with inj_db).
 
-Instance QS_WrapTup {N} : FacadeWrapper ADTValue (@RawTuple (MakeWordHeading N)).
+Instance QS_WrapTuple {N} : FacadeWrapper ADTValue (@RawTuple (MakeWordHeading N)).
 Proof.
   refine {| wrap tp := Tuple (TupleToListW tp);
             wrap_inj := _ |}; Wrapper_t.
@@ -137,12 +142,17 @@ Qed.
 
 Hint Resolve map_TupleToListW_inj : inj_db.
 
-Instance QS_WrapList {N} : FacadeWrapper ADTValue (list (@RawTuple (MakeWordHeading N))).
+Instance QS_WrapTupleList {N} : FacadeWrapper ADTValue (list (@RawTuple (MakeWordHeading N))).
 Proof.
-  refine {| wrap tl := List (List.map TupleToListW tl);
+  refine {| wrap tl := TupleList (List.map TupleToListW tl);
             wrap_inj := _ |}; Wrapper_t.
 Defined.
 
+Instance QS_WrapWordList : FacadeWrapper ADTValue (list W).
+Proof.
+  refine {| wrap tl := WordList tl;
+            wrap_inj := _ |}; Wrapper_t.
+Defined.
 
 Lemma lift_eq {A} (f g: A -> Prop) :
   f = g -> (forall x, f x <-> g x).
@@ -202,6 +212,12 @@ Proof.
             wrap_inj := _ |}; Wrapper_t.
 Defined.
 
+Instance QS_WrapBag2 {N} (M: Word.word 32) (M': Word.word 32) : FacadeWrapper ADTValue (FiatBag N).
+Proof.
+  refine {| wrap tl := Tuples2 (Word.natToWord 32 N) M M' (IndexedEnsemble_TupleToListW tl);
+            wrap_inj := _ |}; Wrapper_t.
+Defined.
+
 Require Import Bedrock.Platform.Facade.examples.QsADTs.
 
 Print Tuple.
@@ -209,235 +225,340 @@ Print TuplesF.tupl.
 
 Print TuplesF.tupl.
 
-(* Require Import CertifiedExtraction.Extraction.External.Core. *)
-(* Require Import Bedrock.Platform.Facade.examples.QsADTs. *)
+Require Import CertifiedExtraction.Extraction.External.Core.
+Require Import Bedrock.Platform.Facade.examples.QsADTs.
 
-(* Section Lists. *)
-(*   Lemma CompileList_new : *)
-(*     forall vret fpointer (env: Env ADTValue) ext tenv N, *)
-(*       GLabelMap.find fpointer env = Some (Axiomatic List_new) -> *)
-(*       vret ∉ ext -> *)
-(*       Lifted_not_mapsto_adt ext tenv vret -> *)
-(*       {{ tenv }} *)
-(*         Call vret fpointer nil *)
-(*         {{ [[ `vret <-- @nil (FiatTuple N) as _ ]] :: DropName vret tenv }} ∪ {{ ext }} // env. *)
-(*   Proof. *)
-(*     repeat (SameValues_Facade_t_step || facade_cleanup_call || LiftPropertyToTelescope_t). *)
-(*     change (ADT (List [])) with (wrap (FacadeWrapper := WrapInstance (H := @QS_WrapList N)) []). *)
-(*     facade_eauto. *)
-(*   Qed. *)
+Section TupleLists.
+  Lemma CompileTupleList_new :
+    forall vret fpointer (env: Env ADTValue) ext tenv N,
+      GLabelMap.find fpointer env = Some (Axiomatic TupleList_new) ->
+      vret ∉ ext ->
+      Lifted_not_mapsto_adt ext tenv vret ->
+      {{ tenv }}
+        Call vret fpointer nil
+      {{ [[ `vret <-- @nil (FiatTuple N) as _ ]] :: DropName vret tenv }} ∪ {{ ext }} // env.
+  Proof.
+    repeat (SameValues_Facade_t_step || facade_cleanup_call || LiftPropertyToTelescope_t).
+    change (ADT (TupleList [])) with (wrap (FacadeWrapper := WrapInstance (H := @QS_WrapTupleList N)) []).
+    facade_eauto.
+  Qed.
 
-(*   Lemma CompileList_delete : *)
-(*     forall vret vlst fpointer (env: Env ADTValue) ext tenv N, *)
-(*       GLabelMap.find fpointer env = Some (Axiomatic List_delete) -> *)
-(*       Lifted_MapsTo ext tenv vlst (wrap (@nil (FiatTuple N))) -> *)
-(*       Lifted_not_mapsto_adt ext tenv vret -> *)
-(*       vret <> vlst -> *)
-(*       vlst ∉ ext -> *)
-(*       vret ∉ ext -> *)
-(*       {{ tenv }} *)
-(*         Call vret fpointer (vlst :: nil) *)
-(*         {{ [[ `vret <-- SCAZero as _ ]] :: DropName vret (DropName vlst tenv) }} ∪ {{ ext }} // env. *)
-(*   Proof. *)
-(*     repeat (SameValues_Facade_t_step || facade_cleanup_call || LiftPropertyToTelescope_t). *)
-(*     facade_eauto. *)
-(*     facade_eauto. *)
-(*   Qed. *)
+  Lemma CompileTupleList_delete :
+    forall vret vlst fpointer (env: Env ADTValue) ext tenv N,
+      GLabelMap.find fpointer env = Some (Axiomatic TupleList_delete) ->
+      Lifted_MapsTo ext tenv vlst (wrap (@nil (FiatTuple N))) ->
+      Lifted_not_mapsto_adt ext tenv vret ->
+      vret <> vlst ->
+      vlst ∉ ext ->
+      vret ∉ ext ->
+      {{ tenv }}
+        Call vret fpointer (vlst :: nil)
+      {{ [[ `vret <-- SCAZero as _ ]] :: DropName vret (DropName vlst tenv) }} ∪ {{ ext }} // env.
+  Proof.
+    repeat (SameValues_Facade_t_step || facade_cleanup_call || LiftPropertyToTelescope_t).
+    facade_eauto.
+    facade_eauto.
+  Qed.
 
-(*   Lemma CompileList_pop : *)
-(*     forall vret vlst fpointer (env: Env ADTValue) ext tenv N *)
-(*       h (t: list (FiatTuple N)), *)
-(*       GLabelMap.find fpointer env = Some (Axiomatic List_pop) -> *)
-(*       Lifted_MapsTo ext tenv vlst (wrap (h :: t)) -> *)
-(*       Lifted_not_mapsto_adt ext tenv vret -> *)
-(*       vret <> vlst -> *)
-(*       vlst ∉ ext -> *)
-(*       vret ∉ ext -> *)
-(*       {{ tenv }} *)
-(*         Call vret fpointer (vlst :: nil) *)
-(*         {{ [[ `vret <-- h as _ ]] :: [[ `vlst <-- t as _ ]] :: DropName vlst (DropName vret tenv) }} ∪ {{ ext }} // env. *)
-(*   Proof. *)
-(*     repeat (SameValues_Facade_t_step || facade_cleanup_call || LiftPropertyToTelescope_t). *)
-(*     facade_eauto. *)
-(*     facade_eauto. *)
-(*     facade_eauto. *)
-(*   Qed. *)
+  Lemma CompileTupleList_pop :
+    forall vret vlst fpointer (env: Env ADTValue) ext tenv N
+      h (t: list (FiatTuple N)),
+      GLabelMap.find fpointer env = Some (Axiomatic TupleList_pop) ->
+      Lifted_MapsTo ext tenv vlst (wrap (h :: t)) ->
+      Lifted_not_mapsto_adt ext tenv vret ->
+      vret <> vlst ->
+      vlst ∉ ext ->
+      vret ∉ ext ->
+      {{ tenv }}
+        Call vret fpointer (vlst :: nil)
+        {{ [[ `vret <-- h as _ ]] :: [[ `vlst <-- t as _ ]] :: DropName vlst (DropName vret tenv) }} ∪ {{ ext }} // env.
+  Proof.
+    repeat (SameValues_Facade_t_step || facade_cleanup_call || LiftPropertyToTelescope_t).
+    facade_eauto.
+    facade_eauto.
+    facade_eauto.
+  Qed.
 
-(*   Lemma CompileList_push : *)
-(*     forall vret vhd vlst fpointer (env: Env ADTValue) ext tenv N *)
-(*       h (t: list (FiatTuple N)), *)
-(*       GLabelMap.find fpointer env = Some (Axiomatic List_push) -> *)
-(*       Lifted_MapsTo ext tenv vhd (wrap h) -> *)
-(*       Lifted_MapsTo ext tenv vlst (wrap t) -> *)
-(*       Lifted_not_mapsto_adt ext tenv vret -> *)
-(*       vret <> vlst -> *)
-(*       vret <> vhd -> *)
-(*       vhd <> vlst -> *)
-(*       vhd ∉ ext -> *)
-(*       vlst ∉ ext -> *)
-(*       vret ∉ ext -> *)
-(*       {{ tenv }} *)
-(*         Call vret fpointer (vlst :: vhd :: nil) *)
-(*         {{ [[ `vret <-- SCAZero as _ ]] :: [[ `vlst <-- h :: t as _ ]] :: DropName vlst (DropName vret (DropName vhd tenv)) }} ∪ {{ ext }} // env. *)
-(*   Proof. *)
-(*     repeat (SameValues_Facade_t_step || facade_cleanup_call || LiftPropertyToTelescope_t). *)
-(*     facade_eauto. *)
-(*     facade_eauto. *)
-(*     facade_eauto. *)
-(*     repeat apply DropName_remove; congruence. *)
-(*   Qed. *)
-(* End Lists. *)
+  Lemma CompileTupleList_push :
+    forall vret vhd vlst fpointer (env: Env ADTValue) ext tenv N
+      h (t: list (FiatTuple N)),
+      GLabelMap.find fpointer env = Some (Axiomatic TupleList_push) ->
+      Lifted_MapsTo ext tenv vhd (wrap h) ->
+      Lifted_MapsTo ext tenv vlst (wrap t) ->
+      Lifted_not_mapsto_adt ext tenv vret ->
+      vret <> vlst ->
+      vret <> vhd ->
+      vhd <> vlst ->
+      vhd ∉ ext ->
+      vlst ∉ ext ->
+      vret ∉ ext ->
+      {{ tenv }}
+        Call vret fpointer (vlst :: vhd :: nil)
+        {{ [[ `vret <-- SCAZero as _ ]] :: [[ `vlst <-- h :: t as _ ]] :: DropName vlst (DropName vret (DropName vhd tenv)) }} ∪ {{ ext }} // env.
+  Proof.
+    repeat (SameValues_Facade_t_step || facade_cleanup_call || LiftPropertyToTelescope_t).
+    facade_eauto.
+    facade_eauto.
+    facade_eauto.
+    repeat apply DropName_remove; congruence.
+  Qed.
+End TupleLists.
 
-(* Section Tuples0. *)
-(*   Definition FiatEmpty N : FiatBag N := fun _ => False. *)
+Definition FiatEmpty N : FiatBag N := fun _ => False.
 
-(*   Lemma Empty_lift: *)
-(*     forall N : nat, *)
-(*       ADT (Tuples0 (Word.natToWord 32 N) Empty) = ADT (Tuples0 (Word.natToWord 32 N) (IndexedEnsemble_TupleToListW (FiatEmpty N))). *)
-(*   Proof. *)
-(*     intros; repeat f_equal. *)
-(*     apply Ensembles.Extensionality_Ensembles. *)
-(*     unfold Ensembles.Same_set, Ensembles.Included, Ensembles.In, FiatEmpty, Empty, IndexedEnsemble_TupleToListW; split; intros. *)
-(*     - exfalso; assumption. *)
-(*     - repeat cleanup. *)
-(*   Qed. *)
+Lemma Empty_lift:
+  forall N : nat,
+    Empty = IndexedEnsemble_TupleToListW (FiatEmpty N).
+Proof.
+  intros; apply Ensembles.Extensionality_Ensembles.
+  unfold Ensembles.Same_set, Ensembles.Included, Ensembles.In, FiatEmpty, Empty, IndexedEnsemble_TupleToListW; split; intros.
+  - exfalso; assumption.
+  - repeat cleanup.
+Qed.
 
-(*   Hint Resolve Empty_lift : call_helpers_db. *)
+Hint Resolve Empty_lift : call_helpers_db.
 
-(*   Lemma CompileTuples0_push : *)
-(*     forall vret vsize fpointer (env: Env ADTValue) ext tenv N, *)
-(*       GLabelMap.find fpointer env = Some (Axiomatic Tuples0_new) -> *)
-(*       Lifted_MapsTo ext tenv vsize (wrap (Word.natToWord 32 N)) -> *)
-(*       Lifted_not_mapsto_adt ext tenv vret -> *)
-(*       vret ∉ ext -> *)
-(*       ~ Word.wlt (Word.natToWord 32 N) (Word.natToWord 32 2) -> *)
-(*       {{ tenv }} *)
-(*         Call vret fpointer (vsize :: nil) *)
-(*       {{ [[ `vret <-- @FiatEmpty N as _ ]] :: DropName vret tenv }} ∪ {{ ext }} // env. *)
-(*   Proof. *)
-(*     repeat (SameValues_Facade_t_step || facade_cleanup_call || LiftPropertyToTelescope_t). *)
-(*     facade_eauto. *)
-(*     facade_eauto. *)
-(*     facade_eauto. *)
-(*   Qed. *)
+Ltac _PreconditionSet_t_in H :=
+  cbv beta iota zeta delta [PreconditionSet PreconditionSet NoDuplicates NoDuplicates_helper] in H; destruct_ands H.
 
-(*   Ltac _PreconditionSet_t_in H := *)
-(*     cbv beta iota zeta delta [PreconditionSet PreconditionSet NoDuplicates NoDuplicates_helper] in H; destruct_ands H. *)
+Ltac _PreconditionSet_t :=
+  cbv beta iota zeta delta [PreconditionSet PreconditionSet_helper NoDuplicates NoDuplicates_helper];
+  repeat match goal with
+         | |- _ /\ _ => split
+         end.
 
-(*   Ltac _PreconditionSet_t := *)
-(*     cbv beta iota zeta delta [PreconditionSet PreconditionSet_helper NoDuplicates NoDuplicates_helper]; *)
-(*     repeat match goal with *)
-(*            | |- _ /\ _ => split *)
-(*            end. *)
+Ltac PreconditionSet_t ::=
+     repeat
+     match goal with
+     | [ H: PreconditionSet _ _ _ |- _ ] => _PreconditionSet_t_in H
+     | [ H: PreconditionSet_helper _ _ _ |- _ ] => _PreconditionSet_t_in H
+     | [ H: NoDuplicates _ |- _ ] => _PreconditionSet_t_in H
+     | [ H: NoDuplicates_helper _ _ |- _ ] => _PreconditionSet_t_in H
+     | [  |- PreconditionSet _ _ _ ] => _PreconditionSet_t
+     | [  |- PreconditionSet_helper _ _ _ ] => _PreconditionSet_t
+     | [  |- NoDuplicates _ ] => _PreconditionSet_t
+     | [  |- NoDuplicates_helper _ _ ] => _PreconditionSet_t
+     end.
 
-(*   Ltac PreconditionSet_t ::= *)
-(*     repeat *)
-(*       match goal with *)
-(*       | [ H: PreconditionSet _ _ _ |- _ ] => _PreconditionSet_t_in H *)
-(*       | [ H: PreconditionSet_helper _ _ _ |- _ ] => _PreconditionSet_t_in H *)
-(*       | [ H: NoDuplicates _ |- _ ] => _PreconditionSet_t_in H *)
-(*       | [ H: NoDuplicates_helper _ _ |- _ ] => _PreconditionSet_t_in H *)
-(*       | [  |- PreconditionSet _ _ _ ] => _PreconditionSet_t *)
-(*       | [  |- PreconditionSet_helper _ _ _ ] => _PreconditionSet_t *)
-(*       | [  |- NoDuplicates _ ] => _PreconditionSet_t *)
-(*       | [  |- NoDuplicates_helper _ _ ] => _PreconditionSet_t *)
-(*       end. *)
+Lemma TupleToListW_length:
+  forall (N : nat) (tuple : FiatTuple N),
+    BinNat.N.lt (BinNat.N.of_nat N) (Word.Npow2 32) ->
+    Datatypes.length (TupleToListW tuple) = Word.wordToNat (Word.natToWord 32 N).
+Proof.
+  intros; rewrite Word.wordToNat_natToWord_idempotent by assumption.
+  clear H.
+  induction N; intros.
+  - destruct tuple; reflexivity.
+  - simpl; f_equal; apply IHN.
+Qed.
 
-(*   Lemma TupleToListW_length: *)
-(*     forall (N : nat) (tuple : FiatTuple N), *)
-(*       BinNat.N.lt (BinNat.N.of_nat N) (Word.Npow2 32) -> *)
-(*       Datatypes.length (TupleToListW tuple) = Word.wordToNat (Word.natToWord 32 N). *)
-(*   Proof. *)
-(*     intros; rewrite Word.wordToNat_natToWord_idempotent by assumption. *)
-(*     clear H. *)
-(*     induction N; intros. *)
-(*     - destruct tuple; reflexivity. *)
-(*     - simpl; f_equal; apply IHN. *)
-(*   Qed. *)
+Hint Resolve TupleToListW_length : call_helpers_db.
 
-(*   Hint Resolve TupleToListW_length : call_helpers_db. *)
-  
-(*   Lemma CompileTuples0_insert : *)
-(*     forall vret vtable vtuple fpointer (env: Env ADTValue) ext tenv N *)
-(*       (table: FiatBag N) (tuple: FiatTuple N), *)
-(*       GLabelMap.find fpointer env = Some (Axiomatic Tuples0_insert) -> *)
-(*       Lifted_MapsTo ext tenv vtable (wrap table) -> *)
-(*       Lifted_MapsTo ext tenv vtuple (wrap tuple) -> *)
-(*       Lifted_not_mapsto_adt ext tenv vret -> *)
-(*       NoDuplicates [[[vret; vtable; vtuple]]] -> *)
-(*       vret ∉ ext -> *)
-(*       vtable ∉ ext -> *)
-(*       vtuple ∉ ext -> *)
-(*       BinNat.N.lt (BinNat.N.of_nat N) (Word.Npow2 32) -> *)
-(*       {{ tenv }} *)
-(*         Call vret fpointer (vtable :: vtuple :: nil) *)
-(*       {{ [[ `vret <-- SCAZero as _ ]] *)
-(*            :: [[ `vtable <-- table as _ ]] *)
-(*            :: DropName vtable (DropName vret (DropName vtuple tenv)) }} ∪ {{ ext }} // env. *)
-(*   Proof. *)
-(*     repeat (SameValues_Facade_t_step || facade_cleanup_call || LiftPropertyToTelescope_t || PreconditionSet_t). *)
+Section Tuples0.
+  Lemma CompileTuples0_new :
+    forall vret vsize fpointer (env: Env ADTValue) ext tenv N,
+      GLabelMap.find fpointer env = Some (Axiomatic Tuples0_new) ->
+      Lifted_MapsTo ext tenv vsize (wrap (Word.natToWord 32 N)) ->
+      Lifted_not_mapsto_adt ext tenv vret ->
+      vret ∉ ext ->
+      ~ Word.wlt (Word.natToWord 32 N) (Word.natToWord 32 2) ->
+      {{ tenv }}
+        Call vret fpointer (vsize :: nil)
+      {{ [[ `vret <-- @FiatEmpty N as _ ]] :: DropName vret tenv }} ∪ {{ ext }} // env.
+  Proof.
+    repeat (SameValues_Facade_t_step || facade_cleanup_call || LiftPropertyToTelescope_t).
+    facade_eauto.
+    repeat f_equal; facade_eauto.
+    facade_eauto.
+  Qed.
 
-(*     Definition FiatBagFunctional {N} (fiatBag: FiatBag N) := *)
-(*       forall t1 t2, *)
-(*         fiatBag t1 -> fiatBag t2 -> *)
-(*         IndexedEnsembles.elementIndex t1 = IndexedEnsembles.elementIndex t2 -> *)
-(*         t1 = t2. *)
+  Lemma CompileTuples0_insert :
+    forall vret vtable vtuple fpointer (env: Env ADTValue) ext tenv N idx
+      (table: FiatBag N) (tuple: FiatTuple N),
+      GLabelMap.find fpointer env = Some (Axiomatic Tuples0_insert) ->
+      Lifted_MapsTo ext tenv vtable (wrap table) ->
+      Lifted_MapsTo ext tenv vtuple (wrap tuple) ->
+      Lifted_not_mapsto_adt ext tenv vret ->
+      NoDuplicates [[[vret; vtable; vtuple]]] ->
+      vret ∉ ext ->
+      vtable ∉ ext ->
+      vtuple ∉ ext ->
+      BinNat.N.lt (BinNat.N.of_nat N) (Word.Npow2 32) ->
+      minFreshIndex (IndexedEnsemble_TupleToListW table) idx ->
+      {{ tenv }}
+        Call vret fpointer (vtable :: vtuple :: nil)
+      {{ [[ `vret <-- SCAZero as _ ]]
+           :: [[ `vtable <-- table as _ ]]
+           :: DropName vtable (DropName vret (DropName vtuple tenv)) }} ∪ {{ ext }} // env.
+  Proof.
+    repeat (SameValues_Facade_t_step || facade_cleanup_call || LiftPropertyToTelescope_t || PreconditionSet_t).
 
-(*     Definition FiatBagMinFreshIndex {N} (fiatBag: FiatBag N) idx := *)
-(*       IndexedEnsembles.UnConstrFreshIdx fiatBag idx /\ *)
-(*       (forall idx' : nat, (lt idx' idx) -> ~ IndexedEnsembles.UnConstrFreshIdx fiatBag idx'). *)
+    (* Definition FiatBagFunctional {N} (fiatBag: FiatBag N) := *)
+    (*   forall t1 t2, *)
+    (*     fiatBag t1 -> fiatBag t2 -> *)
+    (*     IndexedEnsembles.elementIndex t1 = IndexedEnsembles.elementIndex t2 -> *)
+    (*     t1 = t2. *)
 
-(*     Record FiatBag' {N} := *)
-(*       { fiatBag : FiatBag N; *)
-(*         bagFunctional : FiatBagFunctional fiatBag; *)
-(*         idx: nat; *)
-(*         idxIsFresh: FiatBagMinFreshIndex fiatBag idx }. *)
-    
-    
-(*     functional *)
-(*     instantiate (1 := 0); admit. (* FIXME *) *)
+    (* Definition FiatBagMinFreshIndex {N} (fiatBag: FiatBag N) idx := *)
+    (*   IndexedEnsembles.UnConstrFreshIdx fiatBag idx /\ *)
+    (*   (forall idx' : nat, (lt idx' idx) -> ~ IndexedEnsembles.UnConstrFreshIdx fiatBag idx'). *)
 
-(*     facade_eauto. *)
-(*     facade_eauto. *)
-(*     facade_eauto. *)
+    (* Record FiatBag' {N} := *)
+    (*   { fiatBag : FiatBag N; *)
+    (*     bagFunctional : FiatBagFunctional fiatBag; *)
+    (*     idx: nat; *)
+    (*     idxIsFresh: FiatBagMinFreshIndex fiatBag idx }. *)
 
-(*     admit.                      (* FIXME *) *)
-(*     repeat apply DropName_remove; eauto 1. *)
-(*   Qed. *)
+    (* Lemma minFreshIndex_Lift: *)
+    (*   forall (N : nat) (table : FiatBag N) (idx : nat), *)
+    (*     FiatBagMinFreshIndex table idx -> *)
+    (*     minFreshIndex (IndexedEnsemble_TupleToListW table) idx. *)
+    (* Proof. *)
+    (*   unfold FiatBagMinFreshIndex, minFreshIndex. *)
+    (*   repeat cleanup. *)
 
-(*   Lemma CompileTuples0_enumerate : *)
-(*     forall vret vtable fpointer (env: Env ADTValue) ext tenv N *)
-(*       (table: FiatBag N) (tuple: FiatTuple N), *)
-(*       GLabelMap.find fpointer env = Some (Axiomatic Tuples0_enumerate) -> *)
-(*       Lifted_MapsTo ext tenv vtable (wrap table) -> *)
-(*       Lifted_not_mapsto_adt ext tenv vret -> *)
-(*       NoDuplicates [[[vret; vtable]]] -> *)
-(*       vret ∉ ext -> *)
-(*       BinNat.N.lt (BinNat.N.of_nat N) (Word.Npow2 32) -> *)
-(*       {{ tenv }} *)
-(*         Call vret fpointer (vtable :: nil) *)
-(*       {{ [[ `vret <-- @nil (FiatTuple N) as _ ]] :: DropName vret tenv }} ∪ {{ ext }} // env. *)
-(*   Proof. *)
-(*     repeat (SameValues_Facade_t_step || facade_cleanup_call || LiftPropertyToTelescope_t || PreconditionSet_t). *)
-(*     facade_eauto. *)
-(*     admit.                      (* FIXME *) *)
-(*     simpl in H17. *)
-(*     instantiate (1 := 0); admit. (* FIXME *) *)
+    (*   Lemma UnconstrFreshIdx_Lift: *)
+    (*     forall (N : nat) (table : FiatBag N) (idx : nat), *)
+    (*       IndexedEnsembles.UnConstrFreshIdx table idx <-> UnConstrFreshIdx (IndexedEnsemble_TupleToListW table) idx. *)
+    (*   Proof. *)
+    (*     unfold IndexedEnsembles.UnConstrFreshIdx, UnConstrFreshIdx; *)
+    (*     repeat cleanup. *)
+    (*     rewrite <- IndexedElement_RoundTrip in H0. *)
+    (*     pose (IndexedEnsemble_TupleToListW_inj_helpe _ table (IndexedElement_ListWToTuple element)). H0). *)
+    (*   Admitted. *)
 
-(*     facade_eauto. *)
+    (*   apply UnconstrFreshIdx_Lift; assumption. *)
+    (*   rewrite <- UnconstrFreshIdx_Lift. *)
+    (*   eauto. *)
+    (* Qed. *)
 
-(*     repeat apply DropName_remove; eauto 1. *)
-(*   Qed. *)
+    facade_eauto.
+    facade_eauto.
+    facade_eauto.
+    admit.
+    repeat apply DropName_remove; eauto 1.
+  Qed.
 
-  
-(* Lemma CompileTuple_new : *)
-(*   forall vret varg fpointer w (env: Env ADTValue) ext tenv, *)
-(*     Lifted_MapsTo ext tenv varg w -> *)
-(*     {{ tenv }} *)
-(*       Call vret fpointer (varg :: nil) *)
-(*     {{ [[ vret <~~ {tuple:  as _ ]] :: DropName vret tenv }} ∪ {{ext}} // env. *)
-(* Proof. *)
+  Lemma CompileTuples0_enumerate :
+    forall vret vtable fpointer (env: Env ADTValue) ext tenv N
+      (table: FiatBag N) (tuple: FiatTuple N),
+      GLabelMap.find fpointer env = Some (Axiomatic Tuples0_enumerate) ->
+      Lifted_MapsTo ext tenv vtable (wrap table) ->
+      Lifted_not_mapsto_adt ext tenv vret ->
+      NoDuplicates [[[vret; vtable]]] ->
+      vret ∉ ext ->
+      BinNat.N.lt (BinNat.N.of_nat N) (Word.Npow2 32) ->
+      {{ tenv }}
+        Call vret fpointer (vtable :: nil)
+      {{ [[ `vret <-- @nil (FiatTuple N) as _ ]] :: DropName vret tenv }} ∪ {{ ext }} // env.
+  Proof.
+    repeat (SameValues_Facade_t_step || facade_cleanup_call || LiftPropertyToTelescope_t || PreconditionSet_t).
+    facade_eauto.
+    admit.                      (* FIXME *)
+    rewrite <- remove_add_comm by congruence.
+    rewrite <- add_redundant_cancel by eassumption.
+    facade_eauto.
+  Qed.
+End Tuples0.
 
-(*         (* {{ tenv }} *) *)
-(*     (*   InitArgs *) *)
-(*     (* {{ [[`varg <-- N]] :: tenv }} ∪ {{ ext }} // env -> *) *)
+Section Tuples2.
+  Lemma CompileTuples2_new :
+    forall vret vsize vkey1 vkey2 fpointer (env: Env ADTValue) ext tenv N (k1 k2: W),
+      GLabelMap.find fpointer env = Some (Axiomatic Tuples2_new) ->
+      Lifted_MapsTo ext tenv vsize (wrap (Word.natToWord 32 N)) ->
+      Lifted_MapsTo ext tenv vkey1 (wrap k1) ->
+      Lifted_MapsTo ext tenv vkey2 (wrap k2) ->
+      Lifted_not_mapsto_adt ext tenv vret ->
+      vret ∉ ext ->
+      Word.wlt k1 (Word.natToWord 32 N) ->
+      Word.wlt k2 (Word.natToWord 32 N) ->
+      ~ Word.wlt (Word.natToWord 32 N) (Word.natToWord 32 2) ->
+      {{ tenv }}
+        Call vret fpointer (vsize :: vkey1 :: vkey2 :: nil)
+      {{ [[ (NTSome (H := @WrapInstance _ _ (QS_WrapBag2 k1 k2)) vret) <-- @FiatEmpty N as _ ]] :: DropName vret tenv }} ∪ {{ ext }} // env.
+  Proof.
+    repeat (SameValues_Facade_t_step || facade_cleanup_call || LiftPropertyToTelescope_t).
+    facade_eauto.
+    repeat f_equal; facade_eauto.
+    facade_eauto.
+  Qed.
+
+  Lemma CompileTuples2_insert :
+    forall vret vtable vtuple fpointer (env: Env ADTValue) ext tenv N k1 k2 idx
+      (table: FiatBag N) (tuple: FiatTuple N),
+      GLabelMap.find fpointer env = Some (Axiomatic Tuples2_insert) ->
+      Lifted_MapsTo ext tenv vtable (wrap (FacadeWrapper := @WrapInstance _ _ (QS_WrapBag2 k1 k2)) table) ->
+      Lifted_MapsTo ext tenv vtuple (wrap tuple) ->
+      Lifted_not_mapsto_adt ext tenv vret ->
+      NoDuplicates [[[vret; vtable; vtuple]]] ->
+      vret ∉ ext ->
+      vtable ∉ ext ->
+      vtuple ∉ ext ->
+      BinNat.N.lt (BinNat.N.of_nat N) (Word.Npow2 32) ->
+      minFreshIndex (IndexedEnsemble_TupleToListW table) idx ->
+      {{ tenv }}
+        Call vret fpointer (vtable :: vtuple :: nil)
+      {{ [[ `vret <-- SCAZero as _ ]]
+           :: [[ (NTSome (H := @WrapInstance _ _ (QS_WrapBag2 k1 k2)) vtable) <-- table as _ ]]
+           :: DropName vtable (DropName vret (DropName vtuple tenv)) }} ∪ {{ ext }} // env.
+  Proof.
+    repeat (SameValues_Facade_t_step || facade_cleanup_call || LiftPropertyToTelescope_t || PreconditionSet_t).
+    facade_eauto.
+    facade_eauto.
+    facade_eauto.
+    admit.
+    repeat apply DropName_remove; eauto 1.
+  Qed.
+
+  Lemma CompileTuples2_findFirst :
+    forall vret vtable vkey fpointer (env: Env ADTValue) ext tenv N k1 k2
+      (table: FiatBag N) (key: W),
+      GLabelMap.find fpointer env = Some (Axiomatic Tuples2_findFirst) ->
+      Lifted_MapsTo ext tenv vtable (wrap (FacadeWrapper := @WrapInstance _ _ (QS_WrapBag2 k1 k2)) table) ->
+      Lifted_MapsTo ext tenv vkey (wrap key) ->
+      Lifted_not_mapsto_adt ext tenv vret ->
+      NoDuplicates [[[vret; vtable; vkey]]] ->
+      vret ∉ ext ->
+      vtable ∉ ext ->
+      functional (IndexedEnsemble_TupleToListW table) ->
+      {{ tenv }}
+        Call vret fpointer (vtable :: vkey :: nil)
+      {{ [[ `vret <-- @nil (FiatTuple N) as _ ]]
+           :: [[ (NTSome (H := @WrapInstance _ _ (QS_WrapBag2 k1 k2)) vtable) <-- table as _ ]]
+           :: DropName vtable (DropName vret tenv) }} ∪ {{ ext }} // env.
+  Proof.
+    repeat (SameValues_Facade_t_step || facade_cleanup_call || LiftPropertyToTelescope_t || PreconditionSet_t).
+    facade_eauto.
+    facade_eauto.
+    facade_eauto.
+    admit.
+    facade_eauto.
+    repeat apply DropName_remove; eauto 1.
+  Qed.
+
+  Lemma CompileTuples2_findSecond :
+    forall vret vtable vkey fpointer (env: Env ADTValue) ext tenv N k1 k2
+      (table: FiatBag N) (key: W),
+      GLabelMap.find fpointer env = Some (Axiomatic Tuples2_findSecond) ->
+      Lifted_MapsTo ext tenv vtable (wrap (FacadeWrapper := @WrapInstance _ _ (QS_WrapBag2 k1 k2)) table) ->
+      Lifted_MapsTo ext tenv vkey (wrap key) ->
+      Lifted_not_mapsto_adt ext tenv vret ->
+      NoDuplicates [[[vret; vtable; vkey]]] ->
+      vret ∉ ext ->
+      vtable ∉ ext ->
+      functional (IndexedEnsemble_TupleToListW table) ->
+      {{ tenv }}
+        Call vret fpointer (vtable :: vkey :: nil)
+      {{ [[ `vret <-- @nil (FiatTuple N) as _ ]]
+           :: [[ (NTSome (H := @WrapInstance _ _ (QS_WrapBag2 k1 k2)) vtable) <-- table as _ ]]
+           :: DropName vtable (DropName vret tenv) }} ∪ {{ ext }} // env.
+  Proof.
+    repeat (SameValues_Facade_t_step || facade_cleanup_call || LiftPropertyToTelescope_t || PreconditionSet_t).
+    facade_eauto.
+    facade_eauto.
+    facade_eauto.
+    admit.
+    facade_eauto.
+    repeat apply DropName_remove; eauto 1.
+  Qed.
+End Tuples2.
